Nit, before the pause

fairneris/aneris_lang/resources.v
@@ -8,11 +8,10 @@ From fairneris.lib Require Import gen_heap_light.
 From fairneris.aneris_lang Require Export aneris_lang network.
 From fairneris.algebra Require Import disj_gsets.
 From trillium.events Require Import event.
-From fairneris Require Import fairness.
 From fairneris.aneris_lang Require Import events.
 From fairneris.prelude Require Import gset_map.
 From fairneris.lib Require Export singletons.
-From fairneris Require Import fuel fair_resources.
+From fairneris Require Import fairness fuel fair_resources env_model.
 
 Set Default Proof Using "Type".
 
@@ -85,11 +84,16 @@ Definition aneris_localeO := leibnizO aneris_locale.
 Definition live_roleUR (FM : FairModel) :=
   authUR (gset_disjUR $ FM.(fmrole)).
 
+Instance aneris_good: GoodLang aneris_lang.
+Proof. Qed.
+
+(* Instance aneris_inh: Inhabited (action aneris_lang). *)
+
 (** The system CMRA *)
-Class anerisG `{M: FairModel} (FM : LiveModel aneris_lang M) Σ :=
+Class anerisG `(LM : LiveModel aneris_lang (joint_model M Net)) Σ :=
   AnerisG {
       aneris_invG :> invGS_gen HasNoLc Σ;
-      aneris_fairnessG :> fairnessGS FM Σ;
+      aneris_fairnessG :> fairnessGS LM Σ;
       (** global tracking of the ghost names of node-local heaps *)
       aneris_node_gnames_mapG :> inG Σ (authR node_gnames_mapUR);
       aneris_node_gnames_name : gname;
@@ -134,10 +138,10 @@ Class anerisG `{M: FairModel} (FM : LiveModel aneris_lang M) Σ :=
       aneris_observed_recv_name : gname;
     }.
 
-Class anerisPreG `{M: FairModel} (FM : LiveModel aneris_lang M) Σ :=
+Class anerisPreG `(LM : LiveModel aneris_lang (joint_model M Net)) Σ :=
   AnerisPreG {
       anerisPre_invGS :> invGpreS Σ;
-      anerisPre_fairnessGS :> fairnessGpreS FM Σ;
+      anerisPre_fairnessGS :> fairnessGpreS LM Σ;
       anerisPre_node_gnames_mapG :> inG Σ (authR node_gnames_mapUR);
       anerisPre_heapG :> inG Σ (authR local_heapUR);
       anerisPre_socketG :> inG Σ (authR local_socketsUR);
@@ -158,7 +162,7 @@ Class anerisPreG `{M: FairModel} (FM : LiveModel aneris_lang M) Σ :=
         inG Σ (authUR (gmapUR socket_address_group (exclR aneris_eventsO)));
     }.
 
-Definition anerisΣ (M: FairModel) : gFunctors :=
+Definition anerisΣ `(LM : LiveModel aneris_lang (joint_model M Net)) : gFunctors :=
   #[invΣ;
     fairnessΣ aneris_lang M;
     GFunctor (authR node_gnames_mapUR);
@@ -177,12 +181,12 @@ Definition anerisΣ (M: FairModel) : gFunctors :=
     GFunctor (authUR (gmapUR socket_address_group (exclR aneris_eventsO)))
    ].
 
-#[global] Instance subG_anerisPreG {Σ: gFunctors} {M: FairModel} (LM: LiveModel aneris_lang M) :
-  subG (anerisΣ M) Σ → anerisPreG LM Σ.
+#[global] Instance subG_anerisPreG {Σ: gFunctors} `(LM : LiveModel aneris_lang (joint_model M Net)) :
+  subG (anerisΣ LM) Σ → anerisPreG LM Σ.
 Proof. solve_inG. Qed.
 
 Section definitions.
-  Context `{LM: LiveModel aneris_lang M}.
+  Context `{LM: LiveModel aneris_lang (joint_model M Net)}.
   Context `{aG : !anerisG LM Σ}.
 
   (** Authoritative view of the system ghost names *)
@@ -475,7 +479,7 @@ Notation "sa ⤳1[ bs , br ] s" := (sa ⤳1[bs,br]{ 1 } s)%I (at level 20) : bi_
 Notation "sa ⤇1 Φ" := ({[sa]} ⤇* Φ) (at level 20).
 
 Section singleton_to_singleton_connectives.
-  Context `{LM: LiveModel aneris_lang M}.
+  Context `{LM: LiveModel aneris_lang (joint_model M Net)}.
   Context `{aG : !anerisG LM Σ}.
 
   Definition message_history_singleton (sag : socket_address_group) q
@@ -756,7 +760,7 @@ Proof.
   rewrite !bool_decide_eq_true; eauto.
 Qed.
 
-Lemma model_init `{anerisPreG FM Σ} (st : fair_model_to_model FM) :
+Lemma model_init `{anerisPreG FM Σ} (st : live_model_to_model LM) :
   ⊢ |==> ∃ γ, own γ (● Excl' st) ∗ own γ (◯ Excl' st).
 Proof.
   iMod (own_alloc (● Excl' st ⋅ ◯ Excl' st)) as (γ) "[Hfl Hfr]".
